a really complex unfolding lemma for exprD based on well-typedness.
- This seems annoying. perhaps the answer is to
  expose a simplified version of exprD' with
  a complete phase split. it is trivial to write
  equations on this and then it is just a little
  bit annoying to do the phase split explicitly.

src/Ext/ExprLift.v
@@ -1,4 +1,5 @@
 Require Import List.
+Require Import ExtLib.Core.RelDec.
 Require Import ExtLib.Data.ListNth.
 Require Import ExtLib.Tactics.Consider.
 Require Import ExtLib.Tactics.Injection.
@@ -63,11 +64,23 @@ Section typed.
         end
     end.
 
-  Fixpoint lower s l : expr -> option expr :=
+  Definition lower s l : expr -> option expr :=
     match l with
       | 0 => @Some _
       | _ => lower' s l
     end.
+
+  Theorem lower_lower' : forall e s l,
+                           lower s l e = lower' s l e.
+  Proof.
+    unfold lower. destruct l; simpl; auto.
+    clear; revert s.
+    induction e; simpl; intros;
+    repeat match goal with
+             | H : _ |- _ => rewrite <- H
+           end; auto.
+    rewrite <- Minus.minus_n_O. destruct (NPeano.ltb v s); reflexivity.
+  Qed.
 
   Lemma lift'_0 : forall e s, lift' s 0 e = e.
   Proof.
@@ -94,6 +107,164 @@ Section typed.
       | Not e => mentionsU u e
     end.
 
+  Theorem lift_lower : forall e s l,
+                         lower s l (lift s l e) = Some e.
+  Proof.
+    clear; intros.
+    rewrite lower_lower'. rewrite lift_lift'.
+    generalize dependent s. revert l.
+    induction e; simpl; intros;
+    repeat match goal with
+             | H : match ?X with _ => _ end = _ |- _ =>
+               (consider X; try congruence); [ intros ]
+             | H : _ |- _ => erewrite H by eauto
+           end;
+    inv_all; subst; auto.
+    { case_eq (NPeano.ltb v s); simpl; intros.
+      { rewrite H. reflexivity. }
+      { consider (NPeano.ltb v s); try congruence; intros.
+        consider (NPeano.ltb (v + l) s); intros; try solve [ exfalso; omega ].
+        consider (NPeano.ltb (v + l - s) l); intros; try solve [ exfalso; omega ].
+        f_equal. f_equal.
+        rewrite NPeano.Nat.add_sub. auto. } }
+  Qed.
+
+  Theorem lower_lift : forall e e' s l,
+                         lower s l e = Some e' ->
+                         e = lift s l e'.
+  Proof.
+    intros.
+    rewrite lower_lower' in H. rewrite lift_lift'.
+    generalize dependent s. revert l.
+    revert e'.
+    induction e; simpl; intros;
+    repeat match goal with
+             | H : match ?X with _ => _ end = _ |- _ =>
+               (consider X; try congruence); [ intros ]
+             | H : _ |- _ => erewrite H by eauto
+           end;
+    inv_all; subst; auto.
+    consider (NPeano.ltb v s); intros.
+    { inv_all. subst. simpl. consider (NPeano.ltb v s); intros; auto.
+      exfalso; omega. }
+    { consider (NPeano.ltb (v - s) l); try congruence; intros.
+      inv_all; subst. simpl. consider (NPeano.ltb (v - l) s); intros.
+      exfalso. omega. f_equal. rewrite NPeano.Nat.sub_add. auto. omega. }
+  Qed.
+
+  Lemma typeof_expr_lift : forall tfs us vs vs' vs'' e,
+    ExprT.typeof_expr tfs us (vs ++ vs' ++ vs'') (lift (length vs) (length vs') e) = 
+    ExprT.typeof_expr tfs us (vs ++ vs'') e.
+  Proof.
+    clear. intros. rewrite lift_lift'.
+    revert vs.
+    induction e; simpl; intros;
+    repeat match goal with
+             | H : _ |- _ =>
+               erewrite H
+           end; auto.
+    { consider (NPeano.ltb v (length vs)); simpl; intros;
+      repeat ((rewrite nth_error_app_L by omega) ||
+                                                 (rewrite nth_error_app_R by omega)); auto.
+      f_equal. omega. }
+    { change (t :: vs ++ vs' ++ vs'') with
+      ((t :: vs) ++ vs' ++ vs'').
+      rewrite IHe. auto. }
+  Qed.
+
+  Lemma typeof_env_app : forall (a b : EnvI.env (typD ts)),
+    EnvI.typeof_env (a ++ b) = EnvI.typeof_env a ++ EnvI.typeof_env b.
+  Proof.
+    unfold EnvI.typeof_env; intros.
+    rewrite map_app. reflexivity.
+  Qed.
+  Lemma typeof_env_length : forall (a : EnvI.env (typD ts)),
+    length (EnvI.typeof_env a) = length a.
+  Proof.
+    unfold EnvI.typeof_env; intros.
+    rewrite map_length. reflexivity.
+  Qed.
+
+
+  Theorem exprD_lift : forall (fs : functions ts) us vs vs' vs'' e t,
+                         exprD fs us (vs ++ vs' ++ vs'') (lift (length vs) (length vs') e) t =
+                         exprD fs us (vs ++ vs'') e t.
+  Proof.
+    intros. rewrite lift_lift'. revert t; revert vs.
+    induction e; simpl; intros; autorewrite with exprD_rw; auto.
+    { consider (NPeano.ltb v (length vs)); intros.
+      { autorewrite with exprD_rw. unfold EnvI.lookupAs.
+        repeat rewrite nth_error_app_L by auto. reflexivity. }
+      { autorewrite with exprD_rw. unfold EnvI.lookupAs.
+        repeat rewrite nth_error_app_R by omega.
+        replace (v + length vs' - length vs - length vs') with (v - length vs) by omega.
+        reflexivity. } }
+    { repeat rewrite typeof_env_app.
+      repeat rewrite <- typeof_env_length.
+      rewrite <- lift_lift'. rewrite typeof_expr_lift. rewrite lift_lift'.
+      destruct (ExprT.typeof_expr (ExprT.typeof_funcs fs) (EnvI.typeof_env us)
+       (EnvI.typeof_env vs ++ EnvI.typeof_env vs'') e1); auto.
+      destruct t0; auto. repeat rewrite typeof_env_length.
+      rewrite IHe1. rewrite IHe2. reflexivity. }
+    { destruct t0; auto.
+      Require Import ExtLib.Tactics.EqDep.
+      gen_refl.
+      generalize (typeof_expr_eq_exprD_False fs us t0_1 
+                (vs ++ vs' ++ vs'') (lift' (S (length vs)) (length vs') e)
+                t0_2).
+      generalize (typeof_expr_eq_exprD_False fs us t0_1 
+                (vs ++ vs'') e t0_2).
+      repeat rewrite typeof_env_app.
+      replace (ExprT.typecheck_expr (ExprT.typeof_funcs fs) 
+             (EnvI.typeof_env us)
+             (t0_1
+              :: EnvI.typeof_env vs ++
+                 EnvI.typeof_env vs' ++ EnvI.typeof_env vs'')
+             (lift' (S (length vs)) (length vs') e) t0_2)
+        with (ExprT.typecheck_expr (ExprT.typeof_funcs fs) 
+             (EnvI.typeof_env us)
+             ((t0_1
+              :: EnvI.typeof_env vs) ++
+                 EnvI.typeof_env vs' ++ EnvI.typeof_env vs'')
+             (lift' (length (t0_1 :: EnvI.typeof_env vs)) (length (EnvI.typeof_env vs')) e) t0_2).
+      { Check typeof_expr_lift.
+        unfold ExprT.typecheck_expr.
+        rewrite <- lift_lift'.
+        rewrite (typeof_expr_lift (ExprT.typeof_funcs fs) (EnvI.typeof_env us) (t0_1 :: EnvI.typeof_env vs) (EnvI.typeof_env vs') (EnvI.typeof_env vs'') e).
+        simpl in *.
+        intros.
+        destruct (ExprT.typeof_expr (ExprT.typeof_funcs fs) 
+           (EnvI.typeof_env us)
+           (t0_1 :: EnvI.typeof_env vs ++ EnvI.typeof_env vs'') e); auto.
+        consider (typ_eqb t0 t0_2); auto; intros.
+        f_equal.
+        Require Import FunctionalExtensionality.
+        eapply functional_extensionality; intros.
+        generalize dependent (f0 x).
+        generalize dependent (f x).
+        change (existT (typD ts nil) t0_1 x :: vs ++ vs' ++ vs'')
+          with ((existT (typD ts nil) t0_1 x :: vs) ++ vs' ++ vs'').
+        change (existT (typD ts nil) t0_1 x :: vs ++ vs'')
+          with ((existT (typD ts nil) t0_1 x :: vs) ++ vs'').
+        change (S (length vs)) with (length (existT (typD ts nil) t0_1 x :: vs)).
+        specialize (IHe (existT (typD ts nil) t0_1 x :: vs) t0_2).
+        gen_refl.
+        match goal with
+          | H : ?X = _ |- forall x y z w, match ?Y with _ => _ end _ = _ =>
+            change Y with X
+        end.
+        match goal with
+          | |- forall x y z w, match ?Y with _ => _ end _ = match ?X with _ => _ end _ =>
+            destruct Y; destruct X; try congruence
+        end.
+        intros. exfalso; auto. }
+      { f_equal. f_equal.
+        simpl; rewrite typeof_env_length. auto.
+        rewrite typeof_env_length. auto. } }
+    { destruct t0; auto.
+      rewrite IHe1. rewrite IHe2. auto. }
+    { destruct t; auto. rewrite IHe; auto. }
+  Qed.
 
 (*
   Theorem lift_welltyped : forall fs vs vs' us (e : expr) t,
